Factor out StatDb impl and wp proof

src/Examples/StatDb/Impl.v
@@ -1,11 +1,6 @@
 From Coq Require Import List.
 
-Require Import RecoveryRefinement.POCS.
-Require Import Spec.WeakestPreconditions.
-Require Import Spec.WpRefine.
-
-Import RelationNotations.
-Require Import Helpers.RelationRewriting.
+Require Export RecoveryRefinement.POCS.
 
 Module Var.
   Inductive id := Sum | Count.
@@ -77,51 +72,3 @@ Definition impl : LayerImpl Var.Op DB.Op :=
        end;
      recover := Ret tt;
      init := Ret Initialized; |}.
-
-Definition absr : relation DB.l.(State) Var.l.(State) unit :=
-  fun l s _ =>
-    fst s = fold_right plus 0 l /\
-    snd s = length l.
-
-Definition wp : WPSetup Var.dynamics.
-Proof.
-  refine {| op_wp T (op: Var.Op T) :=
-              match op with
-              | Var.Read i => fun post s => post (Var.get i s) s
-              | Var.Write i v => fun post s => post tt (Var.set i v s)
-              end |}.
-  hnf; intros.
-  destruct op; simpl in *; unfold reads, puts in *; propositional.
-  destruct v; eauto.
-Defined.
-
-Definition rf : LayerRefinement Var.l DB.l.
-Proof.
-  refine {| Layer.impl := impl;
-            Layer.absr := absr; |}.
-  - red; intros.
-    split.
-    + eapply (wp.(wp_refine)); intros.
-      destruct s as [sum' count'].
-      unfold absr in H; simpl in *; propositional.
-      destruct op; simpl.
-      * (* read *)
-        unfold puts; descend; intuition eauto.
-        unfold absr; simpl; intuition eauto.
-      * unfold reads; descend; intuition eauto.
-        unfold absr; intuition eauto.
-    + admit. (* rexec refinement *)
-  - red; intros.
-    eapply refine_unfolded; unfold absr; propositional.
-    destruct s as [sum count]; simpl in *; propositional.
-    destruct v.
-    admit. (* recovery transfers crash step *)
-  - (* initialize abstraction *) simpl.
-    Left.
-    unfold and_then, test, rimpl, pure, any, absr; simpl; propositional.
-    descend; intuition eauto.
-    descend; intuition eauto.
-    descend; intuition eauto.
-    simpl; auto.
-    simpl; auto.
-Abort.
