src/Examples/StatDb/WeakestPreconditionProof.v
@@ -1,0 +1,55 @@
+Require Import Examples.StatDb.Impl.
+
+Import RelationNotations.
+Require Import Helpers.RelationRewriting.
+
+Require Import Spec.WeakestPreconditions.
+Require Import Spec.WpRefine.
+
+Definition absr : relation DB.l.(State) Var.l.(State) unit :=
+  fun l s _ =>
+    fst s = fold_right plus 0 l /\
+    snd s = length l.
+
+Definition wp : WPSetup Var.dynamics.
+Proof.
+  refine {| op_wp T (op: Var.Op T) :=
+              match op with
+              | Var.Read i => fun post s => post (Var.get i s) s
+              | Var.Write i v => fun post s => post tt (Var.set i v s)
+              end |}.
+  hnf; intros.
+  destruct op; simpl in *; unfold reads, puts in *; propositional.
+  destruct v; eauto.
+Defined.
+
+Definition rf : LayerRefinement Var.l DB.l.
+Proof.
+  refine {| Layer.impl := impl;
+            Layer.absr := absr; |}.
+  - red; intros.
+    split.
+    + eapply (wp.(wp_refine)); intros.
+      destruct s as [sum' count'].
+      unfold absr in H; simpl in *; propositional.
+      destruct op; simpl.
+      * (* read *)
+        unfold puts; descend; intuition eauto.
+        unfold absr; simpl; intuition eauto.
+      * unfold reads; descend; intuition eauto.
+        unfold absr; intuition eauto.
+    + admit. (* rexec refinement *)
+  - red; intros.
+    eapply refine_unfolded; unfold absr; propositional.
+    destruct s as [sum count]; simpl in *; propositional.
+    destruct v.
+    admit. (* recovery transfers crash step *)
+  - (* initialize abstraction *) simpl.
+    Left.
+    unfold and_then, test, rimpl, pure, any, absr; simpl; propositional.
+    descend; intuition eauto.
+    descend; intuition eauto.
+    descend; intuition eauto.
+    simpl; auto.
+    simpl; auto.
+Abort.
